src/program_proof/memkv/memkv_ghost.v
@@ -1,0 +1,36 @@
+From iris.algebra Require Import gmap lib.mono_nat.
+From iris.proofmode Require Import base tactics classes.
+From Perennial.base_logic Require Import lib.own.
+From iris.bi.lib Require Import fractional.
+From Perennial.program_proof Require Import proof_prelude.
+
+Class kvMapG Σ :=
+  { kv_map_inG :> inG Σ (gmapUR u64 (prodR (fracR) (agreeR (leibnizO (list u8))) )) }.
+
+Definition kvptsto_frac `{!kvMapG Σ} γ (k:u64) (q:Qp) (v:list u8) :=
+  own γ {[ k := ((q / 2)%Qp, to_agree (v: leibnizO (list u8))) ]}.
+
+Definition kvptsto `{!kvMapG Σ} γ k v := kvptsto_frac γ k 1%Qp v.
+
+Section memkv_ghost.
+
+Context `{!kvMapG Σ}.
+
+Lemma kvptsto_agree γ k q v q' v':
+  kvptsto_frac γ k q v -∗
+  kvptsto_frac γ k q' v' -∗
+  ⌜v = v'⌝
+.
+Proof.
+Admitted.
+
+Lemma kvptsto_update v' γ k v1 v2 :
+  kvptsto γ k v1 -∗
+  kvptsto γ k v2 ==∗
+  kvptsto γ k v' ∗
+  kvptsto γ k v'
+.
+Proof.
+Admitted.
+
+End memkv_ghost.
