src/program_proof/memkv/memkv_marshal_move_shard_proof.v
@@ -1,7 +1,7 @@
 From Perennial.program_proof Require Import proof_prelude.
 From Goose.github_com.mit_pdos.gokv Require Import memkv.
 From Perennial.goose_lang Require Import ffi.grove_ffi.
-From Perennial.program_proof Require Export marshal_proof common_proof.
+From Perennial.program_proof Require Export marshal_proof memkv.common_proof.
 
 (*
   Defines Coq request type for shard server MoveShard RPC. Also defines
