src/program_proof/memkv/memkv_marshal_put_proof.v
@@ -1,0 +1,106 @@
+From Perennial.program_proof Require Import proof_prelude.
+From Goose.github_com.mit_pdos.gokv Require Import memkv.
+From Perennial.goose_lang Require Import ffi.grove_ffi.
+From Perennial.program_proof Require Import marshal_proof.
+
+(*
+  Defines Coq request and reply types for shard server Put RPC. Also defines
+  has_encoding for Put Request/Reply and provides WPs for {de|en}codePutRe{ply|quest}()
+ *)
+
+Section memkv_marshal_put_proof.
+
+Context `{!heapG Σ}.
+
+Record PutRequestC := mkPutRequestC {
+  PR_CID : u64;
+  PR_Seq : u64;
+  PR_Key : u64;
+  PR_Value : list u8
+}.
+
+Record PutReplyC := mkPutReplyC {
+  PR_Err : u64;
+}.
+
+Definition own_PutRequest args_ptr args : iProp Σ :=
+  ∃ val_sl,
+  "HCID" ∷ args_ptr ↦[PutRequest.S :: "CID"] #args.(PR_CID) ∗
+  "HSeq" ∷ args_ptr ↦[PutRequest.S :: "Seq"] #args.(PR_Seq) ∗
+  "HKey" ∷ args_ptr ↦[PutRequest.S :: "Key"] #args.(PR_Key) ∗
+  "HValue" ∷ args_ptr ↦[PutRequest.S :: "Value"] (slice_val val_sl) ∗
+  "HValue_sl" ∷ typed_slice.is_slice val_sl byteT 1%Qp args.(PR_Value) ∗
+  "%HseqPositive" ∷ ⌜int.Z args.(PR_Seq) > 0⌝
+.
+
+Definition own_PutReply reply_ptr rep : iProp Σ :=
+  "HErr" ∷ reply_ptr ↦[PutReply.S :: "Err"] #rep.(PR_Err)
+.
+
+Definition has_encoding_PutRequest (data:list u8) (args:PutRequestC) : Prop :=
+  has_encoding data [ EncUInt64 args.(PR_CID) ; EncUInt64 args.(PR_Seq); EncUInt64 args.(PR_Key); EncUInt64 (length args.(PR_Value)) ; EncBytes args.(PR_Value) ].
+
+Definition has_encoding_PutReply (data:list u8) (rep:PutReplyC) :=
+  has_encoding data [ EncUInt64 rep.(PR_Err) ].
+
+Lemma wp_encodePutRequest args_ptr args :
+  {{{
+       own_PutRequest args_ptr args
+  }}}
+    encodePutRequest #args_ptr
+  {{{
+       (reqData:list u8) req_sl, RET (slice_val req_sl); ⌜has_encoding_PutRequest reqData args⌝ ∗
+                                               typed_slice.is_slice req_sl byteT 1%Qp reqData ∗
+                                               own_PutRequest args_ptr args
+  }}}.
+Proof.
+Admitted.
+
+Lemma wp_decodePutRequest req_sl reqData args :
+  {{{
+       ⌜has_encoding_PutRequest reqData args⌝ ∗
+       typed_slice.is_slice req_sl byteT 1%Qp reqData
+  }}}
+    decodePutRequest (slice_val req_sl)
+  {{{
+       (args_ptr:loc), RET #args_ptr; own_PutRequest args_ptr args
+  }}}.
+Proof.
+Admitted.
+
+Lemma has_encoding_PutRequest_inj (reqRaw:list u8) req req' :
+  has_encoding_PutRequest reqRaw req →
+  has_encoding_PutRequest reqRaw req' →
+  req = req'.
+Proof.
+  intros.
+  unfold has_encoding_PutRequest in *.
+Admitted.
+
+Lemma wp_decodePutReply rep rep_sl repData :
+  {{{
+       typed_slice.is_slice rep_sl byteT 1%Qp repData ∗
+       ⌜has_encoding_PutReply repData rep ⌝
+  }}}
+    decodePutReply (slice_val rep_sl)
+  {{{
+       (rep_ptr:loc) , RET #rep_ptr;
+       own_PutReply rep_ptr rep
+  }}}.
+Proof.
+Admitted.
+
+Lemma wp_encodePutReply rep_ptr rep :
+  {{{
+       own_PutReply rep_ptr rep
+  }}}
+    encodePutReply #rep_ptr
+  {{{
+       repData rep_sl , RET (slice_val rep_sl);
+       typed_slice.is_slice rep_sl byteT 1%Qp repData ∗
+       ⌜has_encoding_PutReply repData rep ⌝
+  }}}.
+Proof.
+Admitted.
+
+End memkv_marshal_put_proof.
