src/program_proof/memkv/memkv_move_shard_proof.v
@@ -6,7 +6,7 @@ From Perennial.program_proof.memkv Require Export memkv_shard_definitions memkv_
 
 Section memkv_move_shard_proof.
 
-Context `{!heapG Σ, rpcG Σ GetReplyC}.
+Context `{!heapG Σ, rpcG Σ GetReplyC, kvMapG Σ}.
 
 Lemma wp_MoveShardRPC (s args_ptr:loc) args γsh γ :
   is_MemKVShardServer s γ -∗
@@ -23,7 +23,6 @@ Lemma wp_MoveShardRPC (s args_ptr:loc) args γsh γ :
 Proof.
   iIntros "#His_shard !#" (Φ) "Hpre HΦ".
   iDestruct "Hpre" as "(Hargs & %HsidLe & #Hother_shard)".
-  iNamed "Hargs".
   wp_lam.
   wp_pures.
   iNamed "His_shard".
@@ -34,16 +33,40 @@ Proof.
   wp_pures.
   wp_pures.
 
+  iNamed "Hargs".
   wp_loadField. wp_loadField.
+  (* initialize peer if necessary *)
+  wp_apply (wp_MapGet with "HpeersMap").
+  iIntros (v ok) "[%Hlookup HpeersMap]".
+  wp_pures.
+  wp_if_destruct.
+  { (* need to make a fresh clerk *)
+    wp_loadField.
+    wp_apply (release_spec with "[-HΦ HCID HSeq HSid HDst]").
+    {
+      iFrame "HmuInv Hlocked".
+      iNext.
+      iExists _,_,_, _, _, _, _, _.
+      iExists _, _, _, _.
+      iFrame "HlastReply_structs ∗".
+      done.
+    }
+    (* TODO: annoying to redo rest of proof; annoying also to use wp_If_join if we let go of the lock and reacquire because all of the existentials change *)
+    admit.
+  }
+
   iDestruct (typed_slice.is_slice_small_acc with "HshardMap_sl") as "[HshardMap_small HshardMap_sl]".
 
   assert (∃ b, shardMapping !! int.nat args.(MR_Sid) = Some b) as [? ?].
   {
     eapply list_lookup_lt.
     rewrite HshardMapLength.
-    rewrite /shardOfC /uNSHARD.
-    admit. (* TODO: More mod inequality reasoning *)
+    done.
   }
+
+  wp_pures.
+  wp_loadField.
+  wp_loadField.
   wp_apply (typed_slice.wp_SliceGet with "[$HshardMap_small]").
   { done. }
   iIntros "HshardMap_small".
@@ -64,17 +87,6 @@ Proof.
     }
     wp_pures.
     by iApply "HΦ".
-  }
-  (* have the shard, so we install to the destination *)
-  wp_loadField.
-  wp_loadField.
-  wp_apply (wp_MapGet with "HpeersMap").
-  iIntros (v ok) "[%Hlookup HpeersMap]".
-  wp_pures.
-  wp_if_destruct.
-  { (* need to make a fresh clerk *)
-    (* FIXME: can't let go of lock here; bug in code *)
-    admit.
   }
   (* have a clerk already in peers *)
   wp_pures.
@@ -108,8 +120,7 @@ Proof.
     split.
     { rewrite list_lookup_fmap. rewrite Hkvs_lookup. apply fmap_is_Some.
       naive_solver. }
-    admit.
-    (* FIXME: goose translated the nil as slice.nil, but we want a nil map *)
+    naive_solver.
   }
   iIntros "Hkvss_small".
   wp_pures.
@@ -181,10 +192,25 @@ Proof.
     iApply (big_sepS_impl with "HownShards").
     iModIntro.
     iIntros.
-    rewrite list_lookup_insert_ne; last first.
-    { admit. (* TODO: injectivity of int.nat *) }
-    rewrite list_lookup_insert_ne; last first.
-    { admit. (* TODO: injectivity of int.nat *) }
+
+    assert (x ≠ args.(MR_Sid)).
+    { set_solver. }
+    assert (int.nat x ≠ int.nat args.(MR_Sid)).
+    {
+      destruct (bool_decide (int.Z x = int.Z args.(MR_Sid))) as [|] eqn:X.
+      {
+        apply bool_decide_eq_true in X.
+        apply word.unsigned_inj in X.
+        done.
+      }
+      {
+        apply bool_decide_eq_false in X.
+        word.
+      }
+    }
+
+    rewrite list_lookup_insert_ne; last done.
+    rewrite list_lookup_insert_ne; last done.
     iFrame.
   }
   by iApply "HΦ".
